\paragraph{16.3(1) Connection on a tensor product space}
\beq{
	   \vec\nabla_{\vec X}''\Lambda
	&= \vec\nabla_{\vec X}''(\vec e_a\otimes\vec e'_R\lambda^{aR})
	 = \vec\nabla_{\vec X}\vec e_a\otimes\vec e'_R\lambda^{aR} + \vec\nabla_{\vec X}(\vec e_a\otimes\vec e'_R\lambda^{aR}) \\
	&= \underbrace{X^i\vec e_b\omega^b_{ia}\otimes\vec e'_R\lambda^{aR}}_{b\leftrightarrow a} + \underbrace{\vec e_a\otimes\vec e_S'\omega^S_{iR}\lambda^{aR}X^i}_{S\leftrightarrow R} + \vec e_a\otimes\vec e_R'\underbrace{\d\lambda^{aR}X^i}_{=X^i\partial_i\lambda^{aR}} \\
	&= X^i\vec e_a\otimes\vec e_R'(\partial_i\lambda^{aR}+\omega^a_{ib}\lambda^{bR}+\omega^R_{iS}\lambda^{aS})
}