\subsection{One-Parameter Subgroups and the Exponential Map}

\subsubsection{One-Parameter Subgroups}

\begin{theorem}[20.1]\textbf{(Characterizations of One-Parameter Subgroups)}
\end{theorem}


\begin{proposition}[20.8] \textbf{(Properties of Exponential Map)} Let $\begin{aligned} & \quad \\ 
    & G \quad \, & \text{ Lie group } \\
    & \mathfrak{g} \quad \, & \text{ Lie algebra } \end{aligned}$

\begin{enumerate}
\item[(a)] $\exp: \mathfrak{g} \to g$ smooth
\item[(b)] $\forall \, X \in \mathfrak{g}$, $s,t\in \mathbb{R}$, $\exp{(s+t)}X = \exp{sX}\exp{tX}$
\item[(c)] $\forall \, X \in \mathfrak{g}$, $(\exp{X})^{-1} = \exp{(-X)}$
\item[(d)] $\forall \, X \in \mathfrak{g}$, $n\in \mathbb{Z}$, $(\exp{X})^n = \exp{(nX)}$
\item[(e)] differential $(d\exp)_0:T_0\mathfrak{g} \to T_eG$ is identity, under canonical identifications of both $T_0\mathfrak{g}$ and $T_eG$ with $\mathfrak{g}$ itself.
\item[(f)] $\exp$ restricts to diffeomorphism from some neighborhood of $0$ in $\mathfrak{g}$ to neighborhood of $e$ in $G$.  
\item[(g)] if $\Phi:G\to H$ lie group homomorphism, following commutes



\begin{tikzpicture}
  \matrix (m) [matrix of math nodes, row sep=3em, column sep=2em, minimum width=1em]
  {
 \mathfrak{g}  &   \mathfrak{h}      \\
G     &   H   \\ };
%  \path[-stealth]
\path[->]
  (m-1-1) edge node [above] {$\Phi_*$} (m-1-2)
edge node [left] {$\exp$} (m-2-1)
(m-1-2) edge node [auto] {$\exp$} (m-2-2)
  (m-2-1) edge node [auto] {$\Phi$} (m-2-2);
\end{tikzpicture}

\item[(h)] flow $\theta$ of left-invariant vector field $X$, $\theta_t = R_{\exp{tX}}$
\end{enumerate}
\end{proposition}

\begin{proof}
\begin{enumerate}
\item[(a)]
\item[(b)]
\item[(c)]
\item[(d)]
\item[(e)] Let $X\in \mathfrak{g}$ arbitrary, let $\begin{aligned} & \quad \\ 
  & \sigma: \mathbb{R} \to \mathfrak{g} \\
  & \sigma(t) = tX \\
  & \dot{\sigma}(0) = X \end{aligned}$




\begin{tikzpicture}
  \matrix (m) [matrix of math nodes, row sep=3em, column sep=2em, minimum width=1em]
  {
 \mathfrak{g}  &   G      \\
T_0\mathfrak{g}     &   T_eG   \\ };
%  \path[-stealth]
\path[->]
  (m-1-1) edge node [above] {$\exp$} (m-1-2)
edge node [left] {$$} (m-2-1)
(m-1-2) edge node [auto] {$(d\exp)_0$} (m-2-2)
  (m-2-1) edge node [auto] {$$} (m-2-2);
\end{tikzpicture}

\[
(d\exp )_0(X) = (d\exp )_0(\dot{\sigma}(0)) = (\exp \circ \sigma)'(0) = (\exp{ (tX)})'(0) = \left. \frac{d}{dt} \right|_{t=0} \exp{ (tX)}= X
\]
\item[(f)] $(d\exp )_0 =1$ and so by inverse function thm., $\exists \, (d\exp)_0^{-1}=1^{-1}=1$, and so $\begin{aligned} & \quad \\
  & U \ni 0 \\
  & U \subseteq \mathfrak{g} \end{aligned} \xrightarrow{ \simeq } \begin{aligned} & \quad \\ 
  & V \ni e \\
  & V \subseteq G \end{aligned}$
\end{enumerate}









\end{proof}
